Klas: also expose GPU-side softmax/logsoftmax

dist/Klas_LogSoftmax.cu
@@ -3,7 +3,7 @@
 
 __global__
 /**
-  hoisted when extracting log_softmax_n_f16
+  hoisted when extracting log_softmax_gpu_n_f16
 */
 static void __hoisted_0(uint32_t lena, half *a_)
 {
@@ -14,7 +14,7 @@ static void __hoisted_0(uint32_t lena, half *a_)
 
 __global__
 /**
-  hoisted when extracting log_softmax_n_f16
+  hoisted when extracting log_softmax_gpu_n_f16
 */
 static void __hoisted_1(uint32_t nth, uint32_t lena, half *a_, half *out)
 {
@@ -40,22 +40,20 @@ static void __hoisted_1(uint32_t nth, uint32_t lena, half *a_, half *out)
 
 __global__
 /**
-  hoisted when extracting log_softmax_n_f16
+  hoisted when extracting log_softmax_gpu_n_f16
 */
-static void __hoisted_2(uint32_t lena, half *ga, half sum)
+static void __hoisted_2(uint32_t lena, half *a, half sum)
 {
     if (1024U * blockIdx.x + threadIdx.x < lena) {
-        half x = ga[1024U * blockIdx.x + threadIdx.x];
-        ga[1024U * blockIdx.x + threadIdx.x] = __hsub(x, hlog(sum));
+        half x = a[1024U * blockIdx.x + threadIdx.x];
+        a[1024U * blockIdx.x + threadIdx.x] = __hsub(x, hlog(sum));
     }
 }
 
-void Klas_LogSoftmax_log_softmax_n_f16(uint32_t nth, uint32_t lena, half *a)
+void Klas_LogSoftmax_log_softmax_gpu_n_f16(uint32_t nth, uint32_t lena, half *a)
 {
-    half *ga = (half *) KPR_GPU_ALLOC(2U, lena);
-    MUST(cudaMemcpy(ga, a, 2U * lena, cudaMemcpyHostToDevice));
     half *a_ = (half *) KPR_GPU_ALLOC(2U, lena);
-    MUST(cudaMemcpy(a_, ga, 2U * lena, cudaMemcpyDeviceToDevice));
+    MUST(cudaMemcpy(a_, a, 2U * lena, cudaMemcpyDeviceToDevice));
     KPR_KCALL(__hoisted_0, (lena + 1023U) / 1024U, 1024U, 0U, lena, a_);
     MUST(cudaDeviceSynchronize());
     half *out = (half *) KPR_GPU_ALLOC(2U, 1U);
@@ -69,15 +67,13 @@ void Klas_LogSoftmax_log_softmax_n_f16(uint32_t nth, uint32_t lena, half *a)
     MUST(cudaFree(out));
     half sum = hout;
     MUST(cudaFree(a_));
-    KPR_KCALL(__hoisted_2, (lena + 1023U) / 1024U, 1024U, 0U, lena, ga, sum);
+    KPR_KCALL(__hoisted_2, (lena + 1023U) / 1024U, 1024U, 0U, lena, a, sum);
     MUST(cudaDeviceSynchronize());
-    MUST(cudaMemcpy(a, ga, 2U * lena, cudaMemcpyDeviceToHost));
-    MUST(cudaFree(ga));
 }
 
 __global__
 /**
-  hoisted when extracting log_softmax_n_f32
+  hoisted when extracting log_softmax_gpu_n_f32
 */
 static void __hoisted_3(uint32_t lena, float *a_)
 {
@@ -88,7 +84,7 @@ static void __hoisted_3(uint32_t lena, float *a_)
 
 __global__
 /**
-  hoisted when extracting log_softmax_n_f32
+  hoisted when extracting log_softmax_gpu_n_f32
 */
 static void __hoisted_4(uint32_t nth, uint32_t lena, float *a_, float *out)
 {
@@ -114,22 +110,21 @@ static void __hoisted_4(uint32_t nth, uint32_t lena, float *a_, float *out)
 
 __global__
 /**
-  hoisted when extracting log_softmax_n_f32
+  hoisted when extracting log_softmax_gpu_n_f32
 */
-static void __hoisted_5(uint32_t lena, float *ga, float sum)
+static void __hoisted_5(uint32_t lena, float *a, float sum)
 {
     if (1024U * blockIdx.x + threadIdx.x < lena) {
-        float x = ga[1024U * blockIdx.x + threadIdx.x];
-        ga[1024U * blockIdx.x + threadIdx.x] = x - logf(sum);
+        float x = a[1024U * blockIdx.x + threadIdx.x];
+        a[1024U * blockIdx.x + threadIdx.x] = x - logf(sum);
     }
 }
 
-void Klas_LogSoftmax_log_softmax_n_f32(uint32_t nth, uint32_t lena, float *a)
+void Klas_LogSoftmax_log_softmax_gpu_n_f32(uint32_t nth, uint32_t lena,
+                                           float *a)
 {
-    float *ga = (float *)KPR_GPU_ALLOC(4U, lena);
-    MUST(cudaMemcpy(ga, a, 4U * lena, cudaMemcpyHostToDevice));
     float *a_ = (float *)KPR_GPU_ALLOC(4U, lena);
-    MUST(cudaMemcpy(a_, ga, 4U * lena, cudaMemcpyDeviceToDevice));
+    MUST(cudaMemcpy(a_, a, 4U * lena, cudaMemcpyDeviceToDevice));
     KPR_KCALL(__hoisted_3, (lena + 1023U) / 1024U, 1024U, 0U, lena, a_);
     MUST(cudaDeviceSynchronize());
     float *out = (float *)KPR_GPU_ALLOC(4U, 1U);
@@ -143,15 +138,13 @@ void Klas_LogSoftmax_log_softmax_n_f32(uint32_t nth, uint32_t lena, float *a)
     MUST(cudaFree(out));
     float sum = hout;
     MUST(cudaFree(a_));
-    KPR_KCALL(__hoisted_5, (lena + 1023U) / 1024U, 1024U, 0U, lena, ga, sum);
+    KPR_KCALL(__hoisted_5, (lena + 1023U) / 1024U, 1024U, 0U, lena, a, sum);
     MUST(cudaDeviceSynchronize());
-    MUST(cudaMemcpy(a, ga, 4U * lena, cudaMemcpyDeviceToHost));
-    MUST(cudaFree(ga));
 }
 
 __global__
 /**
-  hoisted when extracting log_softmax_n_f64
+  hoisted when extracting log_softmax_gpu_n_f64
 */
 static void __hoisted_6(uint32_t lena, double *a_)
 {
@@ -162,7 +155,7 @@ static void __hoisted_6(uint32_t lena, double *a_)
 
 __global__
 /**
-  hoisted when extracting log_softmax_n_f64
+  hoisted when extracting log_softmax_gpu_n_f64
 */
 static void __hoisted_7(uint32_t nth, uint32_t lena, double *a_, double *out)
 {
@@ -188,22 +181,21 @@ static void __hoisted_7(uint32_t nth, uint32_t lena, double *a_, double *out)
 
 __global__
 /**
-  hoisted when extracting log_softmax_n_f64
+  hoisted when extracting log_softmax_gpu_n_f64
 */
-static void __hoisted_8(uint32_t lena, double *ga, double sum)
+static void __hoisted_8(uint32_t lena, double *a, double sum)
 {
     if (1024U * blockIdx.x + threadIdx.x < lena) {
-        double x = ga[1024U * blockIdx.x + threadIdx.x];
-        ga[1024U * blockIdx.x + threadIdx.x] = x - log(sum);
+        double x = a[1024U * blockIdx.x + threadIdx.x];
+        a[1024U * blockIdx.x + threadIdx.x] = x - log(sum);
     }
 }
 
-void Klas_LogSoftmax_log_softmax_n_f64(uint32_t nth, uint32_t lena, double *a)
+void Klas_LogSoftmax_log_softmax_gpu_n_f64(uint32_t nth, uint32_t lena,
+                                           double *a)
 {
-    double *ga = (double *)KPR_GPU_ALLOC(8U, lena);
-    MUST(cudaMemcpy(ga, a, 8U * lena, cudaMemcpyHostToDevice));
     double *a_ = (double *)KPR_GPU_ALLOC(8U, lena);
-    MUST(cudaMemcpy(a_, ga, 8U * lena, cudaMemcpyDeviceToDevice));
+    MUST(cudaMemcpy(a_, a, 8U * lena, cudaMemcpyDeviceToDevice));
     KPR_KCALL(__hoisted_6, (lena + 1023U) / 1024U, 1024U, 0U, lena, a_);
     MUST(cudaDeviceSynchronize());
     double *out = (double *)KPR_GPU_ALLOC(8U, 1U);
@@ -217,15 +209,13 @@ void Klas_LogSoftmax_log_softmax_n_f64(uint32_t nth, uint32_t lena, double *a)
     MUST(cudaFree(out));
     double sum = hout;
     MUST(cudaFree(a_));
-    KPR_KCALL(__hoisted_8, (lena + 1023U) / 1024U, 1024U, 0U, lena, ga, sum);
+    KPR_KCALL(__hoisted_8, (lena + 1023U) / 1024U, 1024U, 0U, lena, a, sum);
     MUST(cudaDeviceSynchronize());
-    MUST(cudaMemcpy(a, ga, 8U * lena, cudaMemcpyDeviceToHost));
-    MUST(cudaFree(ga));
 }
 
 __global__
 /**
-  hoisted when extracting log_softmax_f16
+  hoisted when extracting log_softmax_gpu_f16
 */
 static void __hoisted_9(uint32_t lena, half *a_)
 {
@@ -236,7 +226,7 @@ static void __hoisted_9(uint32_t lena, half *a_)
 
 __global__
 /**
-  hoisted when extracting log_softmax_f16
+  hoisted when extracting log_softmax_gpu_f16
 */
 static void __hoisted_10(uint32_t lena, half *a_, half *out)
 {
@@ -262,22 +252,20 @@ static void __hoisted_10(uint32_t lena, half *a_, half *out)
 
 __global__
 /**
-  hoisted when extracting log_softmax_f16
+  hoisted when extracting log_softmax_gpu_f16
 */
-static void __hoisted_11(uint32_t lena, half *ga, half sum)
+static void __hoisted_11(uint32_t lena, half *a, half sum)
 {
     if (1024U * blockIdx.x + threadIdx.x < lena) {
-        half x = ga[1024U * blockIdx.x + threadIdx.x];
-        ga[1024U * blockIdx.x + threadIdx.x] = __hsub(x, hlog(sum));
+        half x = a[1024U * blockIdx.x + threadIdx.x];
+        a[1024U * blockIdx.x + threadIdx.x] = __hsub(x, hlog(sum));
     }
 }
 
-void Klas_LogSoftmax_log_softmax_f16(uint32_t lena, half *a)
+void Klas_LogSoftmax_log_softmax_gpu_f16(uint32_t lena, half *a)
 {
-    half *ga = (half *) KPR_GPU_ALLOC(2U, lena);
-    MUST(cudaMemcpy(ga, a, 2U * lena, cudaMemcpyHostToDevice));
     half *a_ = (half *) KPR_GPU_ALLOC(2U, lena);
-    MUST(cudaMemcpy(a_, ga, 2U * lena, cudaMemcpyDeviceToDevice));
+    MUST(cudaMemcpy(a_, a, 2U * lena, cudaMemcpyDeviceToDevice));
     KPR_KCALL(__hoisted_9, (lena + 1023U) / 1024U, 1024U, 0U, lena, a_);
     MUST(cudaDeviceSynchronize());
     half *out = (half *) KPR_GPU_ALLOC(2U, 1U);
@@ -291,15 +279,13 @@ void Klas_LogSoftmax_log_softmax_f16(uint32_t lena, half *a)
     MUST(cudaFree(out));
     half sum = hout;
     MUST(cudaFree(a_));
-    KPR_KCALL(__hoisted_11, (lena + 1023U) / 1024U, 1024U, 0U, lena, ga, sum);
+    KPR_KCALL(__hoisted_11, (lena + 1023U) / 1024U, 1024U, 0U, lena, a, sum);
     MUST(cudaDeviceSynchronize());
-    MUST(cudaMemcpy(a, ga, 2U * lena, cudaMemcpyDeviceToHost));
-    MUST(cudaFree(ga));
 }
 
 __global__
 /**
-  hoisted when extracting log_softmax_f32
+  hoisted when extracting log_softmax_gpu_f32
 */
 static void __hoisted_12(uint32_t lena, float *a_)
 {
@@ -310,7 +296,7 @@ static void __hoisted_12(uint32_t lena, float *a_)
 
 __global__
 /**
-  hoisted when extracting log_softmax_f32
+  hoisted when extracting log_softmax_gpu_f32
 */
 static void __hoisted_13(uint32_t lena, float *a_, float *out)
 {
@@ -336,22 +322,20 @@ static void __hoisted_13(uint32_t lena, float *a_, float *out)
 
 __global__
 /**
-  hoisted when extracting log_softmax_f32
+  hoisted when extracting log_softmax_gpu_f32
 */
-static void __hoisted_14(uint32_t lena, float *ga, float sum)
+static void __hoisted_14(uint32_t lena, float *a, float sum)
 {
     if (1024U * blockIdx.x + threadIdx.x < lena) {
-        float x = ga[1024U * blockIdx.x + threadIdx.x];
-        ga[1024U * blockIdx.x + threadIdx.x] = x - logf(sum);
+        float x = a[1024U * blockIdx.x + threadIdx.x];
+        a[1024U * blockIdx.x + threadIdx.x] = x - logf(sum);
     }
 }
 
-void Klas_LogSoftmax_log_softmax_f32(uint32_t lena, float *a)
+void Klas_LogSoftmax_log_softmax_gpu_f32(uint32_t lena, float *a)
 {
-    float *ga = (float *)KPR_GPU_ALLOC(4U, lena);
-    MUST(cudaMemcpy(ga, a, 4U * lena, cudaMemcpyHostToDevice));
     float *a_ = (float *)KPR_GPU_ALLOC(4U, lena);
-    MUST(cudaMemcpy(a_, ga, 4U * lena, cudaMemcpyDeviceToDevice));
+    MUST(cudaMemcpy(a_, a, 4U * lena, cudaMemcpyDeviceToDevice));
     KPR_KCALL(__hoisted_12, (lena + 1023U) / 1024U, 1024U, 0U, lena, a_);
     MUST(cudaDeviceSynchronize());
     float *out = (float *)KPR_GPU_ALLOC(4U, 1U);
@@ -365,15 +349,13 @@ void Klas_LogSoftmax_log_softmax_f32(uint32_t lena, float *a)
     MUST(cudaFree(out));
     float sum = hout;
     MUST(cudaFree(a_));
-    KPR_KCALL(__hoisted_14, (lena + 1023U) / 1024U, 1024U, 0U, lena, ga, sum);
+    KPR_KCALL(__hoisted_14, (lena + 1023U) / 1024U, 1024U, 0U, lena, a, sum);
     MUST(cudaDeviceSynchronize());
-    MUST(cudaMemcpy(a, ga, 4U * lena, cudaMemcpyDeviceToHost));
-    MUST(cudaFree(ga));
 }
 
 __global__
 /**
-  hoisted when extracting log_softmax_f64
+  hoisted when extracting log_softmax_gpu_f64
 */
 static void __hoisted_15(uint32_t lena, double *a_)
 {
@@ -384,7 +366,7 @@ static void __hoisted_15(uint32_t lena, double *a_)
 
 __global__
 /**
-  hoisted when extracting log_softmax_f64
+  hoisted when extracting log_softmax_gpu_f64
 */
 static void __hoisted_16(uint32_t lena, double *a_, double *out)
 {
@@ -410,22 +392,20 @@ static void __hoisted_16(uint32_t lena, double *a_, double *out)
 
 __global__
 /**
-  hoisted when extracting log_softmax_f64
+  hoisted when extracting log_softmax_gpu_f64
 */
-static void __hoisted_17(uint32_t lena, double *ga, double sum)
+static void __hoisted_17(uint32_t lena, double *a, double sum)
 {
     if (1024U * blockIdx.x + threadIdx.x < lena) {
-        double x = ga[1024U * blockIdx.x + threadIdx.x];
-        ga[1024U * blockIdx.x + threadIdx.x] = x - log(sum);
+        double x = a[1024U * blockIdx.x + threadIdx.x];
+        a[1024U * blockIdx.x + threadIdx.x] = x - log(sum);
     }
 }
 
-void Klas_LogSoftmax_log_softmax_f64(uint32_t lena, double *a)
+void Klas_LogSoftmax_log_softmax_gpu_f64(uint32_t lena, double *a)
 {
-    double *ga = (double *)KPR_GPU_ALLOC(8U, lena);
-    MUST(cudaMemcpy(ga, a, 8U * lena, cudaMemcpyHostToDevice));
     double *a_ = (double *)KPR_GPU_ALLOC(8U, lena);
-    MUST(cudaMemcpy(a_, ga, 8U * lena, cudaMemcpyDeviceToDevice));
+    MUST(cudaMemcpy(a_, a, 8U * lena, cudaMemcpyDeviceToDevice));
     KPR_KCALL(__hoisted_15, (lena + 1023U) / 1024U, 1024U, 0U, lena, a_);
     MUST(cudaDeviceSynchronize());
     double *out = (double *)KPR_GPU_ALLOC(8U, 1U);
@@ -439,7 +419,449 @@ void Klas_LogSoftmax_log_softmax_f64(uint32_t lena, double *a)
     MUST(cudaFree(out));
     double sum = hout;
     MUST(cudaFree(a_));
-    KPR_KCALL(__hoisted_17, (lena + 1023U) / 1024U, 1024U, 0U, lena, ga, sum);
+    KPR_KCALL(__hoisted_17, (lena + 1023U) / 1024U, 1024U, 0U, lena, a, sum);
+    MUST(cudaDeviceSynchronize());
+}
+
+__global__
+/**
+  hoisted when extracting log_softmax_n_f16
+*/
+static void __hoisted_18(uint32_t lena, half *a_)
+{
+    if (1024U * blockIdx.x + threadIdx.x < lena)
+        a_[1024U * blockIdx.x + threadIdx.x] =
+            hexp(a_[1024U * blockIdx.x + threadIdx.x]);
+}
+
+__global__
+/**
+  hoisted when extracting log_softmax_n_f16
+*/
+static void __hoisted_19(uint32_t nth, uint32_t lena, half *a_, half *out)
+{
+    half *sa = (half *) KPR_SHMEM_AT(0U);
+    half acc = __float2half_rn(0.0f);
+    uint32_t idx = threadIdx.x;
+    for (; idx < lena; idx += nth)
+        acc = __hadd(acc, a_[idx]);
+    sa[threadIdx.x] = acc;
+    uint32_t n = 0U;
+    for (; 1U << (uint32_t) n < nth; n++) {
+        uint32_t __anf01 = n;
+        __syncthreads();
+        uint32_t nextid = threadIdx.x + (uint32_t) (1U << (uint32_t) __anf01);
+        if (nextid < nth)
+            if ((threadIdx.x & (uint32_t) (1U << (uint32_t) (__anf01 + 1U)) -
+                 1U) == 0U)
+                sa[threadIdx.x] = __hadd(sa[threadIdx.x], sa[nextid]);
+    }
+    if (threadIdx.x == 0U)
+        *out = *sa;
+}
+
+__global__
+/**
+  hoisted when extracting log_softmax_n_f16
+*/
+static void __hoisted_20(uint32_t lena, half *ga, half sum)
+{
+    if (1024U * blockIdx.x + threadIdx.x < lena) {
+        half x = ga[1024U * blockIdx.x + threadIdx.x];
+        ga[1024U * blockIdx.x + threadIdx.x] = __hsub(x, hlog(sum));
+    }
+}
+
+void Klas_LogSoftmax_log_softmax_n_f16(uint32_t nth, uint32_t lena, half *a)
+{
+    half *ga = (half *) KPR_GPU_ALLOC(2U, lena);
+    MUST(cudaMemcpy(ga, a, 2U * lena, cudaMemcpyHostToDevice));
+    half *a_ = (half *) KPR_GPU_ALLOC(2U, lena);
+    MUST(cudaMemcpy(a_, ga, 2U * lena, cudaMemcpyDeviceToDevice));
+    KPR_KCALL(__hoisted_18, (lena + 1023U) / 1024U, 1024U, 0U, lena, a_);
+    MUST(cudaDeviceSynchronize());
+    half *out = (half *) KPR_GPU_ALLOC(2U, 1U);
+    KPR_SHMEM_FITS(2U * nth);
+    MUST(cudaFuncSetAttribute
+         (__hoisted_19, cudaFuncAttributeMaxDynamicSharedMemorySize, 2U * nth));
+    KPR_KCALL(__hoisted_19, 1U, nth, 2U * nth, nth, lena, a_, out);
+    MUST(cudaDeviceSynchronize());
+    half hout = __float2half_rn(0.0f);
+    MUST(cudaMemcpy(&hout, out, 2U, cudaMemcpyDeviceToHost));
+    MUST(cudaFree(out));
+    half sum = hout;
+    MUST(cudaFree(a_));
+    KPR_KCALL(__hoisted_20, (lena + 1023U) / 1024U, 1024U, 0U, lena, ga, sum);
+    MUST(cudaDeviceSynchronize());
+    MUST(cudaMemcpy(a, ga, 2U * lena, cudaMemcpyDeviceToHost));
+    MUST(cudaFree(ga));
+}
+
+__global__
+/**
+  hoisted when extracting log_softmax_n_f32
+*/
+static void __hoisted_21(uint32_t lena, float *a_)
+{
+    if (1024U * blockIdx.x + threadIdx.x < lena)
+        a_[1024U * blockIdx.x + threadIdx.x] =
+            expf(a_[1024U * blockIdx.x + threadIdx.x]);
+}
+
+__global__
+/**
+  hoisted when extracting log_softmax_n_f32
+*/
+static void __hoisted_22(uint32_t nth, uint32_t lena, float *a_, float *out)
+{
+    float *sa = (float *)KPR_SHMEM_AT(0U);
+    float acc = 0.0f;
+    uint32_t idx = threadIdx.x;
+    for (; idx < lena; idx += nth)
+        acc += a_[idx];
+    sa[threadIdx.x] = acc;
+    uint32_t n = 0U;
+    for (; 1U << (uint32_t) n < nth; n++) {
+        uint32_t __anf01 = n;
+        __syncthreads();
+        uint32_t nextid = threadIdx.x + (uint32_t) (1U << (uint32_t) __anf01);
+        if (nextid < nth)
+            if ((threadIdx.x & (uint32_t) (1U << (uint32_t) (__anf01 + 1U)) -
+                 1U) == 0U)
+                sa[threadIdx.x] += sa[nextid];
+    }
+    if (threadIdx.x == 0U)
+        *out = *sa;
+}
+
+__global__
+/**
+  hoisted when extracting log_softmax_n_f32
+*/
+static void __hoisted_23(uint32_t lena, float *ga, float sum)
+{
+    if (1024U * blockIdx.x + threadIdx.x < lena) {
+        float x = ga[1024U * blockIdx.x + threadIdx.x];
+        ga[1024U * blockIdx.x + threadIdx.x] = x - logf(sum);
+    }
+}
+
+void Klas_LogSoftmax_log_softmax_n_f32(uint32_t nth, uint32_t lena, float *a)
+{
+    float *ga = (float *)KPR_GPU_ALLOC(4U, lena);
+    MUST(cudaMemcpy(ga, a, 4U * lena, cudaMemcpyHostToDevice));
+    float *a_ = (float *)KPR_GPU_ALLOC(4U, lena);
+    MUST(cudaMemcpy(a_, ga, 4U * lena, cudaMemcpyDeviceToDevice));
+    KPR_KCALL(__hoisted_21, (lena + 1023U) / 1024U, 1024U, 0U, lena, a_);
+    MUST(cudaDeviceSynchronize());
+    float *out = (float *)KPR_GPU_ALLOC(4U, 1U);
+    KPR_SHMEM_FITS(4U * nth);
+    MUST(cudaFuncSetAttribute
+         (__hoisted_22, cudaFuncAttributeMaxDynamicSharedMemorySize, 4U * nth));
+    KPR_KCALL(__hoisted_22, 1U, nth, 4U * nth, nth, lena, a_, out);
+    MUST(cudaDeviceSynchronize());
+    float hout = 0.0f;
+    MUST(cudaMemcpy(&hout, out, 4U, cudaMemcpyDeviceToHost));
+    MUST(cudaFree(out));
+    float sum = hout;
+    MUST(cudaFree(a_));
+    KPR_KCALL(__hoisted_23, (lena + 1023U) / 1024U, 1024U, 0U, lena, ga, sum);
+    MUST(cudaDeviceSynchronize());
+    MUST(cudaMemcpy(a, ga, 4U * lena, cudaMemcpyDeviceToHost));
+    MUST(cudaFree(ga));
+}
+
+__global__
+/**
+  hoisted when extracting log_softmax_n_f64
+*/
+static void __hoisted_24(uint32_t lena, double *a_)
+{
+    if (1024U * blockIdx.x + threadIdx.x < lena)
+        a_[1024U * blockIdx.x + threadIdx.x] =
+            exp(a_[1024U * blockIdx.x + threadIdx.x]);
+}
+
+__global__
+/**
+  hoisted when extracting log_softmax_n_f64
+*/
+static void __hoisted_25(uint32_t nth, uint32_t lena, double *a_, double *out)
+{
+    double *sa = (double *)KPR_SHMEM_AT(0U);
+    double acc = 0.0l;
+    uint32_t idx = threadIdx.x;
+    for (; idx < lena; idx += nth)
+        acc += a_[idx];
+    sa[threadIdx.x] = acc;
+    uint32_t n = 0U;
+    for (; 1U << (uint32_t) n < nth; n++) {
+        uint32_t __anf01 = n;
+        __syncthreads();
+        uint32_t nextid = threadIdx.x + (uint32_t) (1U << (uint32_t) __anf01);
+        if (nextid < nth)
+            if ((threadIdx.x & (uint32_t) (1U << (uint32_t) (__anf01 + 1U)) -
+                 1U) == 0U)
+                sa[threadIdx.x] += sa[nextid];
+    }
+    if (threadIdx.x == 0U)
+        *out = *sa;
+}
+
+__global__
+/**
+  hoisted when extracting log_softmax_n_f64
+*/
+static void __hoisted_26(uint32_t lena, double *ga, double sum)
+{
+    if (1024U * blockIdx.x + threadIdx.x < lena) {
+        double x = ga[1024U * blockIdx.x + threadIdx.x];
+        ga[1024U * blockIdx.x + threadIdx.x] = x - log(sum);
+    }
+}
+
+void Klas_LogSoftmax_log_softmax_n_f64(uint32_t nth, uint32_t lena, double *a)
+{
+    double *ga = (double *)KPR_GPU_ALLOC(8U, lena);
+    MUST(cudaMemcpy(ga, a, 8U * lena, cudaMemcpyHostToDevice));
+    double *a_ = (double *)KPR_GPU_ALLOC(8U, lena);
+    MUST(cudaMemcpy(a_, ga, 8U * lena, cudaMemcpyDeviceToDevice));
+    KPR_KCALL(__hoisted_24, (lena + 1023U) / 1024U, 1024U, 0U, lena, a_);
+    MUST(cudaDeviceSynchronize());
+    double *out = (double *)KPR_GPU_ALLOC(8U, 1U);
+    KPR_SHMEM_FITS(8U * nth);
+    MUST(cudaFuncSetAttribute
+         (__hoisted_25, cudaFuncAttributeMaxDynamicSharedMemorySize, 8U * nth));
+    KPR_KCALL(__hoisted_25, 1U, nth, 8U * nth, nth, lena, a_, out);
+    MUST(cudaDeviceSynchronize());
+    double hout = 0.0l;
+    MUST(cudaMemcpy(&hout, out, 8U, cudaMemcpyDeviceToHost));
+    MUST(cudaFree(out));
+    double sum = hout;
+    MUST(cudaFree(a_));
+    KPR_KCALL(__hoisted_26, (lena + 1023U) / 1024U, 1024U, 0U, lena, ga, sum);
+    MUST(cudaDeviceSynchronize());
+    MUST(cudaMemcpy(a, ga, 8U * lena, cudaMemcpyDeviceToHost));
+    MUST(cudaFree(ga));
+}
+
+__global__
+/**
+  hoisted when extracting log_softmax_f16
+*/
+static void __hoisted_27(uint32_t lena, half *a_)
+{
+    if (1024U * blockIdx.x + threadIdx.x < lena)
+        a_[1024U * blockIdx.x + threadIdx.x] =
+            hexp(a_[1024U * blockIdx.x + threadIdx.x]);
+}
+
+__global__
+/**
+  hoisted when extracting log_softmax_f16
+*/
+static void __hoisted_28(uint32_t lena, half *a_, half *out)
+{
+    half *sa = (half *) KPR_SHMEM_AT(0U);
+    half acc = __float2half_rn(0.0f);
+    uint32_t idx = threadIdx.x;
+    for (; idx < lena; idx += 1024U)
+        acc = __hadd(acc, a_[idx]);
+    sa[threadIdx.x] = acc;
+    uint32_t n = 0U;
+    for (; 1U << (uint32_t) n < 1024U; n++) {
+        uint32_t __anf01 = n;
+        __syncthreads();
+        uint32_t nextid = threadIdx.x + (uint32_t) (1U << (uint32_t) __anf01);
+        if (nextid < 1024U)
+            if ((threadIdx.x & (uint32_t) (1U << (uint32_t) (__anf01 + 1U)) -
+                 1U) == 0U)
+                sa[threadIdx.x] = __hadd(sa[threadIdx.x], sa[nextid]);
+    }
+    if (threadIdx.x == 0U)
+        *out = *sa;
+}
+
+__global__
+/**
+  hoisted when extracting log_softmax_f16
+*/
+static void __hoisted_29(uint32_t lena, half *ga, half sum)
+{
+    if (1024U * blockIdx.x + threadIdx.x < lena) {
+        half x = ga[1024U * blockIdx.x + threadIdx.x];
+        ga[1024U * blockIdx.x + threadIdx.x] = __hsub(x, hlog(sum));
+    }
+}
+
+void Klas_LogSoftmax_log_softmax_f16(uint32_t lena, half *a)
+{
+    half *ga = (half *) KPR_GPU_ALLOC(2U, lena);
+    MUST(cudaMemcpy(ga, a, 2U * lena, cudaMemcpyHostToDevice));
+    half *a_ = (half *) KPR_GPU_ALLOC(2U, lena);
+    MUST(cudaMemcpy(a_, ga, 2U * lena, cudaMemcpyDeviceToDevice));
+    KPR_KCALL(__hoisted_27, (lena + 1023U) / 1024U, 1024U, 0U, lena, a_);
+    MUST(cudaDeviceSynchronize());
+    half *out = (half *) KPR_GPU_ALLOC(2U, 1U);
+    KPR_SHMEM_FITS(2048U);
+    MUST(cudaFuncSetAttribute
+         (__hoisted_28, cudaFuncAttributeMaxDynamicSharedMemorySize, 2048U));
+    KPR_KCALL(__hoisted_28, 1U, 1024U, 2048U, lena, a_, out);
+    MUST(cudaDeviceSynchronize());
+    half hout = __float2half_rn(0.0f);
+    MUST(cudaMemcpy(&hout, out, 2U, cudaMemcpyDeviceToHost));
+    MUST(cudaFree(out));
+    half sum = hout;
+    MUST(cudaFree(a_));
+    KPR_KCALL(__hoisted_29, (lena + 1023U) / 1024U, 1024U, 0U, lena, ga, sum);
+    MUST(cudaDeviceSynchronize());
+    MUST(cudaMemcpy(a, ga, 2U * lena, cudaMemcpyDeviceToHost));
+    MUST(cudaFree(ga));
+}
+
+__global__
+/**
+  hoisted when extracting log_softmax_f32
+*/
+static void __hoisted_30(uint32_t lena, float *a_)
+{
+    if (1024U * blockIdx.x + threadIdx.x < lena)
+        a_[1024U * blockIdx.x + threadIdx.x] =
+            expf(a_[1024U * blockIdx.x + threadIdx.x]);
+}
+
+__global__
+/**
+  hoisted when extracting log_softmax_f32
+*/
+static void __hoisted_31(uint32_t lena, float *a_, float *out)
+{
+    float *sa = (float *)KPR_SHMEM_AT(0U);
+    float acc = 0.0f;
+    uint32_t idx = threadIdx.x;
+    for (; idx < lena; idx += 1024U)
+        acc += a_[idx];
+    sa[threadIdx.x] = acc;
+    uint32_t n = 0U;
+    for (; 1U << (uint32_t) n < 1024U; n++) {
+        uint32_t __anf01 = n;
+        __syncthreads();
+        uint32_t nextid = threadIdx.x + (uint32_t) (1U << (uint32_t) __anf01);
+        if (nextid < 1024U)
+            if ((threadIdx.x & (uint32_t) (1U << (uint32_t) (__anf01 + 1U)) -
+                 1U) == 0U)
+                sa[threadIdx.x] += sa[nextid];
+    }
+    if (threadIdx.x == 0U)
+        *out = *sa;
+}
+
+__global__
+/**
+  hoisted when extracting log_softmax_f32
+*/
+static void __hoisted_32(uint32_t lena, float *ga, float sum)
+{
+    if (1024U * blockIdx.x + threadIdx.x < lena) {
+        float x = ga[1024U * blockIdx.x + threadIdx.x];
+        ga[1024U * blockIdx.x + threadIdx.x] = x - logf(sum);
+    }
+}
+
+void Klas_LogSoftmax_log_softmax_f32(uint32_t lena, float *a)
+{
+    float *ga = (float *)KPR_GPU_ALLOC(4U, lena);
+    MUST(cudaMemcpy(ga, a, 4U * lena, cudaMemcpyHostToDevice));
+    float *a_ = (float *)KPR_GPU_ALLOC(4U, lena);
+    MUST(cudaMemcpy(a_, ga, 4U * lena, cudaMemcpyDeviceToDevice));
+    KPR_KCALL(__hoisted_30, (lena + 1023U) / 1024U, 1024U, 0U, lena, a_);
+    MUST(cudaDeviceSynchronize());
+    float *out = (float *)KPR_GPU_ALLOC(4U, 1U);
+    KPR_SHMEM_FITS(4096U);
+    MUST(cudaFuncSetAttribute
+         (__hoisted_31, cudaFuncAttributeMaxDynamicSharedMemorySize, 4096U));
+    KPR_KCALL(__hoisted_31, 1U, 1024U, 4096U, lena, a_, out);
+    MUST(cudaDeviceSynchronize());
+    float hout = 0.0f;
+    MUST(cudaMemcpy(&hout, out, 4U, cudaMemcpyDeviceToHost));
+    MUST(cudaFree(out));
+    float sum = hout;
+    MUST(cudaFree(a_));
+    KPR_KCALL(__hoisted_32, (lena + 1023U) / 1024U, 1024U, 0U, lena, ga, sum);
+    MUST(cudaDeviceSynchronize());
+    MUST(cudaMemcpy(a, ga, 4U * lena, cudaMemcpyDeviceToHost));
+    MUST(cudaFree(ga));
+}
+
+__global__
+/**
+  hoisted when extracting log_softmax_f64
+*/
+static void __hoisted_33(uint32_t lena, double *a_)
+{
+    if (1024U * blockIdx.x + threadIdx.x < lena)
+        a_[1024U * blockIdx.x + threadIdx.x] =
+            exp(a_[1024U * blockIdx.x + threadIdx.x]);
+}
+
+__global__
+/**
+  hoisted when extracting log_softmax_f64
+*/
+static void __hoisted_34(uint32_t lena, double *a_, double *out)
+{
+    double *sa = (double *)KPR_SHMEM_AT(0U);
+    double acc = 0.0l;
+    uint32_t idx = threadIdx.x;
+    for (; idx < lena; idx += 1024U)
+        acc += a_[idx];
+    sa[threadIdx.x] = acc;
+    uint32_t n = 0U;
+    for (; 1U << (uint32_t) n < 1024U; n++) {
+        uint32_t __anf01 = n;
+        __syncthreads();
+        uint32_t nextid = threadIdx.x + (uint32_t) (1U << (uint32_t) __anf01);
+        if (nextid < 1024U)
+            if ((threadIdx.x & (uint32_t) (1U << (uint32_t) (__anf01 + 1U)) -
+                 1U) == 0U)
+                sa[threadIdx.x] += sa[nextid];
+    }
+    if (threadIdx.x == 0U)
+        *out = *sa;
+}
+
+__global__
+/**
+  hoisted when extracting log_softmax_f64
+*/
+static void __hoisted_35(uint32_t lena, double *ga, double sum)
+{
+    if (1024U * blockIdx.x + threadIdx.x < lena) {
+        double x = ga[1024U * blockIdx.x + threadIdx.x];
+        ga[1024U * blockIdx.x + threadIdx.x] = x - log(sum);
+    }
+}
+
+void Klas_LogSoftmax_log_softmax_f64(uint32_t lena, double *a)
+{
+    double *ga = (double *)KPR_GPU_ALLOC(8U, lena);
+    MUST(cudaMemcpy(ga, a, 8U * lena, cudaMemcpyHostToDevice));
+    double *a_ = (double *)KPR_GPU_ALLOC(8U, lena);
+    MUST(cudaMemcpy(a_, ga, 8U * lena, cudaMemcpyDeviceToDevice));
+    KPR_KCALL(__hoisted_33, (lena + 1023U) / 1024U, 1024U, 0U, lena, a_);
+    MUST(cudaDeviceSynchronize());
+    double *out = (double *)KPR_GPU_ALLOC(8U, 1U);
+    KPR_SHMEM_FITS(8192U);
+    MUST(cudaFuncSetAttribute
+         (__hoisted_34, cudaFuncAttributeMaxDynamicSharedMemorySize, 8192U));
+    KPR_KCALL(__hoisted_34, 1U, 1024U, 8192U, lena, a_, out);
+    MUST(cudaDeviceSynchronize());
+    double hout = 0.0l;
+    MUST(cudaMemcpy(&hout, out, 8U, cudaMemcpyDeviceToHost));
+    MUST(cudaFree(out));
+    double sum = hout;
+    MUST(cudaFree(a_));
+    KPR_KCALL(__hoisted_35, (lena + 1023U) / 1024U, 1024U, 0U, lena, ga, sum);
     MUST(cudaDeviceSynchronize());
     MUST(cudaMemcpy(a, ga, 8U * lena, cudaMemcpyDeviceToHost));
     MUST(cudaFree(ga));
