dist/Klas_LogSoftmax.h
@@ -4,6 +4,21 @@
 
 #include <kuiper.h>
 
+void Klas_LogSoftmax_log_softmax_gpu_n_f16(uint32_t nth, uint32_t lena,
+                                           half * a);
+
+void Klas_LogSoftmax_log_softmax_gpu_n_f32(uint32_t nth, uint32_t lena,
+                                           float *a);
+
+void Klas_LogSoftmax_log_softmax_gpu_n_f64(uint32_t nth, uint32_t lena,
+                                           double *a);
+
+void Klas_LogSoftmax_log_softmax_gpu_f16(uint32_t lena, half * a);
+
+void Klas_LogSoftmax_log_softmax_gpu_f32(uint32_t lena, float *a);
+
+void Klas_LogSoftmax_log_softmax_gpu_f64(uint32_t lena, double *a);
+
 void Klas_LogSoftmax_log_softmax_n_f16(uint32_t nth, uint32_t lena, half * a);
 
 void Klas_LogSoftmax_log_softmax_n_f32(uint32_t nth, uint32_t lena, float *a);
