src/lib/kernel/Kuiper.Kernel.LogSoftmax.fsti
@@ -7,10 +7,31 @@ open Kuiper.Seq.Common
 module SZ = Kuiper.SizeT
 module Vec = Pulse.Lib.Vec
 module SM = Kuiper.Kernel.Softmax
+module Array1 = Kuiper.Array1
+open Kuiper.Array1
+open Kuiper.Tensor.Layout.Alg { l1_forward }
 
 // Log of softmax.
 let log_softmax_real (s:Seq.seq real { Seq.length s > 0 }) =
   lseq_map rlog (seq_refine (fun x -> x >. 0.0R) (SM.softmax_real s))
+
+unfold
+type log_softmax_gpu_ty (et : Type0) {| floating et, real_like et |} =
+  fn (nth : szp{nth <= max_threads})
+     (#lena : szp)
+     (a : array1 et (l1_forward lena) { is_global a })
+     (#va : erased (lseq et lena))
+     (ra : erased (lseq real lena))
+  preserves
+    cpu
+  requires
+    on gpu_loc (a |-> va) **
+    pure (va %~ ra) **
+    pure (lena <= max_blocks * max_threads)
+  ensures
+    exists* (va' : lseq et lena).
+      on gpu_loc (a |-> va') **
+      pure (va' %~ log_softmax_real ra)
 
 unfold
 type log_softmax_ty (et : Type0) {| floating et, real_like et |} =
@@ -30,6 +51,10 @@ type log_softmax_ty (et : Type0) {| floating et, real_like et |} =
     exists* (va' : lseq et lena).
       a |-> va' **
       pure (va' %~ log_softmax_real ra)
+
+inline_for_extraction noextract
+val log_softmax_gpu (#et : Type0) {| floating et, real_like et, floating_real_like et |}
+  : log_softmax_gpu_ty et
 
 inline_for_extraction noextract
 val log_softmax (#et : Type0) {| floating et, real_like et, floating_real_like et |}
