src/lib/kernel/Kuiper.Kernel.Softmax.fsti
@@ -6,11 +6,32 @@ open Kuiper.Real { rexp }
 open Kuiper.Seq.Common
 module SZ = Kuiper.SizeT
 module Vec = Pulse.Lib.Vec
+module Array1 = Kuiper.Array1
+open Kuiper.Array1
+open Kuiper.Tensor.Layout.Alg { l1_forward }
 
 let softmax_real (s:Seq.seq real { Seq.length s > 0 }) =
   let exps = seq_map rexp s in
   let summ : real = rsum exps in
   seq_map (fun x -> rexp x /. summ) s
+
+unfold
+type softmax_gpu_ty (et : Type0) {| floating et, real_like et |} =
+  fn (nth : szp{nth <= max_threads})
+     (#lena : szp)
+     (a : array1 et (l1_forward lena) { is_global a })
+     (#va : erased (lseq et lena))
+     (ra : erased (lseq real lena))
+  preserves
+    cpu
+  requires
+    on gpu_loc (a |-> va) **
+    pure (va %~ ra) **
+    pure (lena <= max_blocks * max_threads)
+  ensures
+    exists* (va' : lseq et lena).
+      on gpu_loc (a |-> va') **
+      pure (va' %~ softmax_real ra)
 
 unfold
 type softmax_ty (et : Type0) {| floating et, real_like et |} =
@@ -30,6 +51,10 @@ type softmax_ty (et : Type0) {| floating et, real_like et |} =
     exists* (va' : lseq et lena).
       a |-> va' **
       pure (va' %~ softmax_real ra)
+
+inline_for_extraction noextract
+val softmax_gpu (#et : Type0) {| floating et, real_like et, floating_real_like et |}
+  : softmax_gpu_ty et
 
 inline_for_extraction noextract
 val softmax (#et : Type0) {| floating et, real_like et, floating_real_like et |}
