src/klas/Klas.LogSoftmax.fst
@@ -5,6 +5,16 @@ open Kuiper
 
 module K = Kuiper.Kernel.LogSoftmax
 
+(* GPU-pointer variants, dynamic thread number *)
+let log_softmax_gpu_n_f16 : K.log_softmax_gpu_ty f16 = K.log_softmax_gpu
+let log_softmax_gpu_n_f32 : K.log_softmax_gpu_ty f32 = K.log_softmax_gpu
+let log_softmax_gpu_n_f64 : K.log_softmax_gpu_ty f64 = K.log_softmax_gpu
+
+(* GPU-pointer variants, full blocks *)
+let log_softmax_gpu_f16 lena = K.log_softmax_gpu #f16 1024sz #lena
+let log_softmax_gpu_f32 lena = K.log_softmax_gpu #f32 1024sz #lena
+let log_softmax_gpu_f64 lena = K.log_softmax_gpu #f64 1024sz #lena
+
 (* dynamic thread number *)
 let log_softmax_n_f16 : K.log_softmax_ty f16 = K.log_softmax
 let log_softmax_n_f32 : K.log_softmax_ty f32 = K.log_softmax
