src/klas/Klas.Softmax.fsti
@@ -4,6 +4,10 @@ module Klas.Softmax
 open Kuiper
 module K = Kuiper.Kernel.Softmax
 
+val softmax_gpu_n_f16 : K.softmax_gpu_ty f16
+val softmax_gpu_n_f32 : K.softmax_gpu_ty f32
+val softmax_gpu_n_f64 : K.softmax_gpu_ty f64
+
 val softmax_n_f16 : K.softmax_ty f16
 val softmax_n_f32 : K.softmax_ty f32
 val softmax_n_f64 : K.softmax_ty f64
